wip

src/drf/DRF_PF.v
@@ -50,59 +50,16 @@ Inductive promised (mem: Memory.t) (loc: Loc.t) (to: Time.t) : Prop :=
     promised mem loc to
 .
 
-Inductive promised_loc (mem: Memory.t) (loc: Loc.t) : Prop :=
-| promised_loc_intro
-    to
-    (PROMISED: promised mem loc to)
-  :
-    promised_loc mem loc
+Inductive forget_memory P msrc mtgt : Prop :=
+| forget_memory_intro
+    (* (FUTURE: Memory.le msrc mtgt) *)
+    (COMPLETE: forall l t (NPROMS: ~ P l t),
+        Memory.get l t msrc = Memory.get l t mtgt)
+    (FORGET: forall l t (PROMS: P l t), Memory.get l t msrc = None)
 .
-
-Inductive all_promises (c: Configuration.t) (P: IdentMap.key -> Prop)
-          (l: Loc.t) (t: Time.t) : Prop :=
-| all_promises_intro
-    tid st lc
-    (TID1: IdentMap.find tid c.(Configuration.threads) = Some (st, lc))
-    (PROMISED: promised lc.(Local.promises) l t)
-    (SAT: P tid)
-.
-
-Module Forget.
-
-  Inductive forget_statelocal:
-    sigT Language.state * Local.t -> sigT Language.state * Local.t -> Prop :=
-  | forget_statelocal_intro
-      st lc1 lc2
-      (TVIEW : lc1.(Local.tview) = lc2.(Local.tview))
-      (PROMS : lc1.(Local.promises) = Memory.bot)
-    :
-      forget_statelocal (st, lc1) (st, lc2)
-  .
-
-  Inductive forget_memory P msrc mtgt : Prop :=
-  | forget_memory_intro
-      (* (FUTURE: Memory.le msrc mtgt) *)
-      (COMPLETE: forall l t (NPROMS: ~ P l t),
-          Memory.get l t msrc = Memory.get l t mtgt)
-      (FORGET: forall l t (PROMS: P l t), Memory.get l t msrc = None)
-  .
-  
-  Inductive forget_config csrc ctgt : Prop :=
-  | forget_configuration_intro
-      (THS : forall tid, option_rel
-                           forget_statelocal 
-                           (IdentMap.find tid csrc.(Configuration.threads))
-                           (IdentMap.find tid ctgt.(Configuration.threads)))
-      (SC : csrc.(Configuration.sc) = ctgt.(Configuration.sc))
-      (MEM : forget_memory
-               (all_promises ctgt (fun _ => True))
-               csrc.(Configuration.memory) ctgt.(Configuration.memory))
-  .
-  
-End Forget.
 
 Lemma forget_memory_le P msrc mtgt
-      (FORGET: Forget.forget_memory P msrc mtgt)
+      (FORGET: forget_memory P msrc mtgt)
   :
     Memory.le msrc mtgt.
 Proof.
@@ -146,37 +103,6 @@ Proof.
   + eauto.
   + i. des; clarify. eauto.
 Qed.
-
-Module Inv.
-  
-  Inductive t lang (st: Language.state lang) lc
-            (proms: Memory.t) (updates : Loc.t -> Prop) (mlast: Memory.t): Prop :=
-  | inv_intro
-      (PROMS: forall
-          l m sc (PROM : promised_loc proms l)
-          (FUTURE: unchanged_on
-                     ((fun loc to => covered loc to proms) \2/ (fun loc _ => updates loc))
-                     mlast m),          
-          exists st' lc' sc' m',
-            (<<STEPS : rtc (tau (@Thread.program_step _))
-                           (Thread.mk _ st lc sc m)
-                           (Thread.mk _ st' lc' sc' m')>>) /\
-            (<<WRITING : is_writing _ st' l Ordering.relaxed>>))
-      (UPDATE : forall
-          l m sc (UPD : updates l)
-          (FUTURE: unchanged_on
-                     ((fun loc to => covered loc to proms) \2/ (fun loc _ => updates loc))
-                     mlast m),          
-          exists st' lc' sc' m',
-            (<<STEPS : rtc (tau (@Thread.program_step _))
-                           (Thread.mk _ st lc sc m)
-                           (Thread.mk _ st' lc' sc' m')>>) /\
-            (<<READING : is_reading _ st' l Ordering.relaxed>>)
-      (* /\ (<<WRITING : is_reading _ st' l Ordering.acqrel>>) *)
-      )
-  .
-
-End Inv.
 
 Inductive opt_pred_step P (lang : Language.t)
   : ThreadEvent.t -> Thread.t lang -> Thread.t lang -> Prop :=
@@ -348,10 +274,10 @@ Qed.
 
 Lemma self_promise_remove_promise
       prom prom' mem_src mem_tgt mem_tgt' loc from to msg kind
-      (MEM: Forget.forget_memory (promised prom) mem_src mem_tgt)
+      (MEM: forget_memory (promised prom) mem_src mem_tgt)
       (PROMISE: Memory.promise prom mem_tgt loc from to msg prom' mem_tgt' kind)
   :
-    Forget.forget_memory (promised prom') mem_src mem_tgt'.
+    forget_memory (promised prom') mem_src mem_tgt'.
 Proof.
   dup MEM. eapply forget_memory_le in MEM0. inv MEM. inv PROMISE.
   - econs; eauto.
@@ -478,13 +404,13 @@ Definition no_acq_read_msgs (MSGS : Loc.t -> Time.t -> Prop)
 .
   
 Lemma consistent_certification_no_sc
-      lang th_tgt th_tgt' st st' v v' prom prom' sc sc'
+      P lang th_tgt th_tgt' st st' v v' prom prom' sc sc'
       mem_tgt mem_tgt' e_tgt
       (SCMAX: ~ promise_view_consistent prom sc)
       (TH_TGT0: th_tgt = Thread.mk lang st (Local.mk v Memory.bot) sc mem_tgt)
       (TH_TGT1: th_tgt' = Thread.mk lang st' (Local.mk v' prom') sc' mem_tgt')
       (CONSISTENT: promise_view_consistent prom v'.(TView.cur).(View.rlx))
-      (STEP: (@pred_step (no_promise) lang) e_tgt th_tgt th_tgt')
+      (STEP: (@pred_step (P /1\ no_promise) lang) e_tgt th_tgt th_tgt')
   :
     no_sc e_tgt.
 Proof.
@@ -583,7 +509,7 @@ Lemma self_promise_remove_write v prom v' prom'
                 (Local.mk v prom) sc mem_tgt
                 loc from to val releasedm released ord
                 (Local.mk v' prom') sc' mem_tgt' kind)
-      (MEM: Forget.forget_memory (promised prom) mem_src mem_tgt)
+      (MEM: forget_memory (promised prom) mem_src mem_tgt)
       (LCWF: Local.wf (Local.mk v prom) mem_tgt)
   :
     exists mem_src',
@@ -591,7 +517,7 @@ Lemma self_promise_remove_write v prom v' prom'
                   (Local.mk v Memory.bot) sc mem_src
                   loc from to val releasedm released ord
                   (Local.mk v' Memory.bot) sc' mem_src' Memory.op_kind_add>>) /\
-      (<<MEM: Forget.forget_memory (promised prom') mem_src' mem_tgt'>>).
+      (<<MEM: forget_memory (promised prom') mem_src' mem_tgt'>>).
 Proof.
   dup MEM. eapply forget_memory_le in MEM0. inv MEM.
   inv WRITE. ss. clarify.
@@ -669,7 +595,7 @@ Lemma self_promise_remove
       (TH_SRC: th_src = Thread.mk lang st (Local.mk v Memory.bot) sc mem_src)
       (TH_TGT0: th_tgt = Thread.mk lang st (Local.mk v prom) sc mem_tgt)
       (TH_TGT1: th_tgt' = Thread.mk lang st' (Local.mk v' prom') sc' mem_tgt')
-      (MEM: Forget.forget_memory (promised prom) mem_src mem_tgt)
+      (MEM: forget_memory (promised prom) mem_src mem_tgt)
       (LCWF: Local.wf (Local.mk v prom) mem_tgt)
       (CLOSED: Memory.closed mem_tgt)
   :
@@ -678,7 +604,7 @@ Lemma self_promise_remove
                  (P /1\ no_promise) e_src th_src
                  (Thread.mk lang st' (Local.mk v' Memory.bot) sc' mem_src')>>) /\
       (<<EVT: ThreadEvent.get_event e_src = ThreadEvent.get_event e_tgt>>) /\
-      (<<MEM: Forget.forget_memory (promised prom') mem_src' mem_tgt'>>).
+      (<<MEM: forget_memory (promised prom') mem_src' mem_tgt'>>).
 Proof.
   dup MEM. eapply forget_memory_le in MEM0.  
   clarify. inv STEP. des. inv STEP0. inv STEP.
@@ -738,7 +664,7 @@ Lemma other_promise_remove_write v v' prom'
                 (Local.mk v Memory.bot) sc mem_tgt
                 loc from to val releasedm released ord
                 (Local.mk v' prom') sc' mem_tgt' kind)
-      (MEM: Forget.forget_memory others mem_src mem_tgt)
+      (MEM: forget_memory others mem_src mem_tgt)
       (OTHERS: ~ others loc to)
   :
     exists mem_src',
@@ -746,7 +672,7 @@ Lemma other_promise_remove_write v v' prom'
                   (Local.mk v Memory.bot) sc mem_src
                   loc from to val releasedm released ord
                   (Local.mk v' Memory.bot) sc' mem_src' Memory.op_kind_add>>) /\
-      (<<MEM: Forget.forget_memory others mem_src' mem_tgt'>>).
+      (<<MEM: forget_memory others mem_src' mem_tgt'>>).
 Proof.
   exploit write_msg_wf; eauto. i. des.
   inv WRITE. ss. clarify. exploit memory_write_bot_add; eauto. i. clarify.
@@ -769,18 +695,18 @@ Qed.
 Lemma other_promise_remove
       P lang th_src th_tgt th_tgt' st st' v v' prom' sc sc'
       mem_src mem_tgt mem_tgt' e_tgt others
-      (STEP: (@pred_step (P /1\ no_promise /1\ no_read_msgs others /1\ write_not_in others) lang) e_tgt th_tgt th_tgt')
+      (STEP: (@pred_step (P /1\ no_read_msgs others /1\ write_not_in others /1\ no_promise) lang) e_tgt th_tgt th_tgt')
       (TH_SRC: th_src = Thread.mk lang st (Local.mk v Memory.bot) sc mem_src)
       (TH_TGT0: th_tgt = Thread.mk lang st (Local.mk v Memory.bot) sc mem_tgt)
       (TH_TGT1: th_tgt' = Thread.mk lang st' (Local.mk v' prom') sc' mem_tgt')
-      (MEM: Forget.forget_memory others mem_src mem_tgt)
+      (MEM: forget_memory others mem_src mem_tgt)
   :
     exists mem_src',
       (<<STEP: (@pred_step
-                  (P /1\ no_promise /1\ no_read_msgs others) lang)
+                  (P /1\ no_promise) lang)
                  e_tgt th_src
                  (Thread.mk lang st' (Local.mk v' Memory.bot) sc' mem_src')>>) /\
-      (<<MEM: Forget.forget_memory others mem_src' mem_tgt'>>).
+      (<<MEM: forget_memory others mem_src' mem_tgt'>>).
 Proof.
   dup MEM. eapply forget_memory_le in MEM0.  
   clarify. inv STEP. des. inv STEP0. inv STEP.
@@ -794,13 +720,13 @@ Proof.
     inv MEM. erewrite COMPLETE; eauto.
   - ss. exploit other_promise_remove_write; eauto.
     { exploit write_msg_wf; eauto. i. des.
-      eapply SAT0. econs; eauto. refl. }
+      eapply SAT1. econs; eauto. refl. }
     i. des. exists mem_src'. esplits; eauto.
     econs; eauto. econs; eauto. econs 2; eauto. econs; eauto.
   - ss. inv LOCAL1. ss.
     exploit other_promise_remove_write; eauto.
     { exploit write_msg_wf; eauto. i. des.
-      eapply SAT0. econs; eauto. refl. }
+      eapply SAT1. econs; eauto. refl. }
     i. des. exists mem_src'. esplits; eauto.
     econs; eauto. econs; eauto. econs 2; eauto. econs; eauto.
     econs; eauto. econs; eauto. inv MEM. erewrite COMPLETE; eauto.
@@ -1555,14 +1481,14 @@ Qed.
 Lemma unchanged_on_step
       P L lang th_src th_tgt th_tgt' st st' v v' prom' sc sc'
       mem_src mem_tgt mem_tgt' e_tgt
-      (STEP: (@pred_step (P /1\ no_promise /1\ write_in L) lang) e_tgt th_tgt th_tgt')
+      (STEP: (@pred_step (P /1\ write_in L /1\ no_promise) lang) e_tgt th_tgt th_tgt')
       (TH_SRC: th_src = Thread.mk lang st (Local.mk v Memory.bot) sc mem_src)
       (TH_TGT0: th_tgt = Thread.mk lang st (Local.mk v Memory.bot) sc mem_tgt)
       (TH_TGT1: th_tgt' = Thread.mk lang st' (Local.mk v' prom') sc' mem_tgt')
       (MEM: unchanged_on L mem_tgt mem_src)
   :
     exists mem_src',
-      (<<STEP: (@pred_step (P /1\ no_promise /1\ write_in L) lang)
+      (<<STEP: (@pred_step (P /1\ write_in L /1\ no_promise) lang)
                  e_tgt th_src
                  (Thread.mk lang st' (Local.mk v' Memory.bot) sc' mem_src')>>) /\
       (<<MEM: unchanged_on L mem_tgt' mem_src'>>).
@@ -1610,72 +1536,9 @@ Inductive capped (mem_src mem_tgt: Memory.t): Prop :=
           (<<TOLE: Time.le to_src to>>) /\
           (<<VIEWLE: View.opt_le released_src released>>))
 .
-      
-Inductive sim_pf
-          (mlast: Ident.t -> Memory.t) (updates: Ident.t -> (Loc.t -> Prop))
-          (c_src c_tgt: Configuration.t) : Prop :=
-| sim_pf_intro
-    (FORGET: Forget.forget_config c_src c_tgt)
-    (RACEFREE: pf_racefree c_src)
-    (INV:
-       forall
-         tid lang_src st_src lc_src lang_tgt st_tgt lc_tgt
-         (TIDSRC: IdentMap.find tid c_src.(Configuration.threads) =
-                  Some (existT _ lang_src st_src, lc_src))
-         (TIDTGT: IdentMap.find tid c_tgt.(Configuration.threads) =
-                  Some (existT _ lang_tgt st_tgt, lc_tgt)),
-         Inv.t _ st_src lc_src lc_tgt.(Local.promises) (updates tid) (mlast tid))
-    (FUTURE:
-       forall tid lang_src st_src lc_src
-              (TIDSRC: IdentMap.find tid c_src.(Configuration.threads) =
-                       Some (existT _ lang_src st_src, lc_src)),
-         unchanged_on
-           (fun loc _ => (updates tid) loc)
-           (mlast tid) c_src.(Configuration.memory))
-    (WFSRC: Configuration.wf c_src)
-    (WFTGT: Configuration.wf c_tgt)
-.
-
-Inductive sim_pf_all c_src c_tgt: Prop :=
-| sim_pf_all_intro mlast updates (SIM : sim_pf mlast updates c_src c_tgt)
-.
-
-Lemma init_pf s tid st lc
-      (TID: IdentMap.find tid (Threads.init s) = Some (st, lc))
-  :
-    Local.promises lc = Memory.bot.
-Proof.
-  unfold Threads.init in *. erewrite UsualFMapPositive.UsualPositiveMap.Facts.map_o in *.
-  unfold option_map in *. des_ifs.
-Qed.  
-  
-Lemma sim_pf_init
-      s
-      (RACEFREE: pf_racefree (Configuration.init s))
-  :
-    sim_pf_all (Configuration.init s) (Configuration.init s)
-.
-Proof.
-  econs. instantiate (1:=fun _ _ => False). instantiate (1:=fun _ => Memory.init).
-  econs; eauto; ss; i.
-  - econs; i; ss.
-    + unfold Threads.init in *. erewrite UsualFMapPositive.UsualPositiveMap.Facts.map_o in *.
-      unfold option_map in *. des_ifs.      
-    + econs; ss; eauto. ii. inv PROMS. ss.
-      exploit init_pf; eauto. i. rewrite x0 in *.
-      inv PROMISED. rewrite Memory.bot_get in *. clarify.
-  - econs; s.
-    + i. exploit init_pf; try apply TIDTGT; eauto. i.
-      rewrite x0 in *. inv PROM. inv PROMISED.
-      rewrite Memory.bot_get in *. clarify.
-    + i. clarify.
-  - econs; eauto. refl.
-  - eapply Configuration.init_wf.
-  - eapply Configuration.init_wf.
-Qed. 
 
 Lemma forget_exists_list l mem_tgt:
-  exists mem_src, <<FORGET: Forget.forget_memory (fun loc to => List.In (loc, to) l)
+  exists mem_src, <<FORGET: forget_memory (fun loc to => List.In (loc, to) l)
                                                  mem_src mem_tgt>>.
 Proof.
   induction l; ss.
@@ -1693,7 +1556,7 @@ Proof.
 Qed.
   
 Lemma forget_exists prom mem_tgt:
-  exists mem_src, <<FORGET: Forget.forget_memory prom.(promised) mem_src mem_tgt>>.
+  exists mem_src, <<FORGET: forget_memory prom.(promised) mem_src mem_tgt>>.
 Proof.
   hexploit (Memory.finite_sound_exists prom); eauto. i. des.
   hexploit (forget_exists_list dom mem_tgt). i. des. exists mem_src.
@@ -1827,8 +1690,8 @@ Proof.
   - ii. eapply Memory.add_get1; eauto.
 Qed.
     
-Lemma write_not_in_unchanged_on L e lang (th0 th1: Thread.t lang)
-      (STEP: pred_step (no_promise /1\ write_not_in L) e th0 th1)
+Lemma write_not_in_unchanged_on P L e lang (th0 th1: Thread.t lang)
+      (STEP: pred_step (P /1\ write_not_in L /1\ no_promise) e th0 th1)
       (BOT: th0.(Thread.local).(Local.promises) = Memory.bot)
   :
     unchanged_on L th0.(Thread.memory) th1.(Thread.memory).
@@ -1889,36 +1752,6 @@ Next Obligation.
   ii. exploit COMPLETE0; eauto. i. des.
   exploit COMPLETE; eauto.
 Qed.
-
-(* Inductive shorter_memory (mem_src mem_tgt: Memory.t): Prop := *)
-(* | shorter_memory_intro *)
-(*     (SOUND: forall l t msg_src (GET: Memory.get l t mem_src = Some msg_src), *)
-(*         exists msg_tgt, Memory.get l t mem_tgt = Some msg_tgt) *)
-(*     (COMPLETE: forall loc to from_tgt msg *)
-(*                       (GET: Memory.get loc to mem_tgt = Some (from_tgt, msg)), *)
-(*         exists from_src, *)
-(*           (<<GET: Memory.get loc to mem_src = Some (from_src, msg)>>) /\ *)
-(*           (<<ITV: forall t (IN: Interval.mem (from_src, to) t), *)
-(*               Interval.mem (from_tgt, to) t>>)). *)
-
-(* Lemma shorter_memory_covered mem_src mem_tgt *)
-(*       (SHORTER: shorter_memory mem_src mem_tgt) *)
-(*       l t *)
-(*       (COVER: covered l t mem_src) *)
-(*   : *)
-(*     covered l t mem_tgt. *)
-(* Proof. *)
-(*   inv SHORTER. inv COVER. *)
-(*   exploit SOUND; eauto. i. des. destruct msg_tgt. *)
-(*   exploit COMPLETE; eauto. i. des. clarify. *)
-(*   econs; eauto. *)
-(* Qed. *)
-
-(* Definition not_attatched (L: Loc.t -> Time.t -> Prop) (m: Memory.t) := *)
-(*   forall loc to (SAT: L loc to), *)
-(*   exists to', *)
-(*     (<<TLE: Time.lt to to'>>) /\  *)
-(*     (<<EMPTY: forall l t (ITV: Interval.mem (to, to') t), ~ covered l t m>>). *)
 
 Definition not_attatched (L: Loc.t -> Time.t -> Prop) (m: Memory.t) :=
   forall loc to (SAT: L loc to),
@@ -2070,21 +1903,22 @@ Proof.
 Qed.
 
 Lemma no_update_on_step
-      L lang th_src th_tgt th_tgt' st st' v v' prom' sc sc'
-      mem_tgt mem_tgt' mem_src e
-      (STEP: (@pred_step (no_promise /1\ no_update_on L) lang) e th_tgt th_tgt')
+      P L0 L1 lang th_src th_tgt th_tgt' st st' v v' prom' sc sc'
+      mem_tgt mem_tgt' mem_src e_tgt
+      (STEP: (@pred_step (P /1\ write_not_in L0 /1\ no_update_on L1 /1\ no_promise) lang) e_tgt th_tgt th_tgt')
       (TH_SRC: th_src = Thread.mk lang st (Local.mk v Memory.bot) sc mem_src)
       (TH_TGT0: th_tgt = Thread.mk lang st (Local.mk v Memory.bot) sc mem_tgt)
       (TH_TGT1: th_tgt' = Thread.mk lang st' (Local.mk v' prom') sc' mem_tgt')
       (SHORTER: shorter_memory mem_src mem_tgt)
-      (NOATTATCH: not_attatched L mem_src) 
+      (NOATTATCH: not_attatched L1 mem_src) 
   :
     exists e_src mem_src',
-      (<<STEP: (@pred_step (no_promise) lang)
+      (<<STEP: (@pred_step ((fun _ => True) /1\ write_not_in L0 /1\ no_promise) lang)
                  e_src th_src
                  (Thread.mk lang st' (Local.mk v' prom') sc' mem_src')>>) /\
+      (<<EVT: ThreadEvent.get_event e_src = ThreadEvent.get_event e_tgt>>) /\
       (<<SHORTER: shorter_memory mem_src' mem_tgt'>>) /\
-      (<<NOATTATCH: not_attatched L mem_src'>>).
+      (<<NOATTATCH: not_attatched L1 mem_src'>>).
 Proof.
   dup SHORTER. inv SHORTER. inv STEP. inv STEP0. des. inv STEP.
   - inv STEP0. ss.
@@ -2105,7 +1939,10 @@ Proof.
       { instantiate (1:=Time.middle from to). left. auto. }
       { auto. }
       i. des. esplits; eauto.
-      * econs; eauto. econs; eauto. econs 2; eauto. econs; eauto.
+      * econs; eauto.
+        { econs; eauto. econs 2; eauto. econs; eauto. }
+        ss. esplits; eauto. i. eapply SAT2; eauto.
+        inv IN; ss. econs; eauto.
       * eapply not_attatch_write; eauto. ii.
         exploit NOATTATCH; eauto. i. des.
         exploit memory_add_cover_disjoint; auto.
@@ -2136,1096 +1973,153 @@ Proof.
     + inv LOCAL0. exists (ThreadEvent.fence ordr ordw).
       ss. clarify. esplits; eauto. econs; eauto.
       econs; eauto. econs 2; eauto. econs; eauto.
-    + inv LOCAL0. exists (ThreadEvent.syscall e0).
+    + inv LOCAL0. exists (ThreadEvent.syscall e).
       ss. clarify. esplits; eauto. econs; eauto.
       econs; eauto. econs 2; eauto. econs; eauto.
 Qed.
 
-
-
-
-
-WIP
-
-Lemma not_attatch L prom mem_src mem_tgt loc from1 to1 val released mem_tgt' from'
-      (SHORTER: shorter_memory mem_src mem_tgt)
-      (NOATTATCH: not_attatched L mem_src) 
-      (ADD: Memory.write Memory.bot mem_tgt loc from1 to1 val released prom mem_tgt' Memory.op_kind_add)
+Inductive forget_statelocal:
+  sigT Language.state * Local.t -> sigT Language.state * Local.t -> Prop :=
+| forget_statelocal_intro
+    st lc1 lc2
+    (TVIEW : lc1.(Local.tview) = lc2.(Local.tview))
+    (PROMS : lc1.(Local.promises) = Memory.bot)
   :
-    exists mem_src' to',
-      (<<ADD: Memory.write Memory.bot mem_src loc from' to' val released prom mem_src' Memory.op_kind_add>>) /\  
-      (<<SHORTER: shorter_memory mem_src' mem_tgt'>>) /\
-      (<<NOATTATCH: not_attatched L mem_src'>>).
-Proof.
-
-  
-  dup SHORTER. inv SHORTER. inv ADD. inv PROMISE.
-  exploit MemoryFacts.MemoryFacts.add_remove_eq; try apply REMOVE; eauto. i. clarify.
-  exploit write_succeed; eauto.
-  - instantiate (1:=mem_src). instantiate (1:=loc).
-    ii. eapply COVER in COVER0. inv COVER0.
-    dup MEM. eapply Memory.add_get0 in MEM. des. 
-    dup GET. eapply Memory.add_get1 in GET; eauto.
-    exploit Memory.get_disjoint.
-    + eapply GET.
-    + eapply GET1.
-    + i. des; clarify.
-      eapply x0; eauto. inv H. econs; ss; eauto.
-      eapply TimeFacts.le_lt_lt; eauto.
-  - inv MEM. inv ADD. inv MSG_WF. inv TS. eauto.
-  - inv MEM. inv ADD. eauto.
-  - i. des. inv WRITE. inv PROMISE. esplits; eauto. econs.
-    + i. erewrite Memory.add_o in GET; eauto.      
-      erewrite Memory.add_o; cycle 1; eauto. des_ifs; eauto.
-    + i. inv COV. erewrite Memory.add_o in GET; eauto. des_ifs.
-      * ss; des; clarify. eapply Memory.add_get0 in MEM. des.
-        econs; eauto. inv ITV. econs; eauto.
-        ss. eapply TimeFacts.le_lt_lt; eauto.
-      * exploit COVER.
-        { econs; eauto. }
-        intros COV. inv COV. eapply Memory.add_get1 in GET0; eauto.
-        econs; eauto.
-Qed.
-
-
-Lemma no_update_on_step
-      L lang th_src th_tgt th_tgt' st st' v v' prom' sc sc'
-      mem_tgt mem_tgt' mem_src e
-      (STEP: (@pred_step (no_promise /1\ no_update_on L) lang) e th_tgt th_tgt')
-      (TH_SRC: th_src = Thread.mk lang st (Local.mk v Memory.bot) sc mem_src)
-      (TH_TGT0: th_tgt = Thread.mk lang st (Local.mk v Memory.bot) sc mem_tgt)
-      (TH_TGT1: th_tgt' = Thread.mk lang st' (Local.mk v' prom') sc' mem_tgt')
-      (SHORTER: shorter_memory mem_src mem_tgt)
-      (NOATTATCH: not_attatched L mem_src) 
-  :
-    exists e_src mem_src',
-      (<<STEP: (@pred_step (no_promise) lang)
-                 e_src th_src
-                 (Thread.mk lang st' (Local.mk v' prom') sc' mem_src')>>) /\
-      (<<SHORTER: shorter_memory mem_src' mem_tgt'>>) /\
-      (<<NOATTATCH: not_attatched L mem_src'>>).
-Proof.
-  dup SHORTER. inv SHORTER. inv STEP. inv STEP0. des. inv STEP.
-  - inv STEP0. ss.
-  - inv STEP0. inv LOCAL.
-    + exists mem_src; eauto. econs; eauto. econs; eauto.
-      econs; eauto. econs 2; eauto. econs; eauto.
-    + inv LOCAL0. ss. clarify. exploit COMPLETE; eauto. i. des.
-      exists mem_src; eauto. econs; eauto. econs; eauto.
-      econs; eauto. econs 2; eauto. econs; eauto.
-    + exploit write_msg_wf; eauto. i. des.
-      inv LOCAL0. ss. clarify.
-      exploit memory_write_bot_add; eauto. i. clarify.
-      dup WRITE. exploit shorter_memory_write; eauto.
-      { refl. }
-      i. des. esplits; eauto. econs; eauto. econs; eauto.
-      econs 2; eauto. econs; eauto.
-    + inv LOCAL1. ss. exploit write_msg_wf; eauto. i. des.
-      exploit COMPLETE; eauto. i. des.
-      inv LOCAL2. ss. clarify.
-      exploit memory_write_bot_add; eauto. i. clarify.
-      dup WRITE. exploit shorter_memory_write; eauto.
-      { refl. }
-      i. des. esplits; eauto. econs; eauto. econs; eauto.
-      econs 2; eauto. econs; eauto.
-    + inv LOCAL0. ss. clarify. esplits; eauto. econs; eauto.
-      econs; eauto. econs 2; eauto. econs; eauto.
-    + inv LOCAL0. ss. clarify. esplits; eauto. econs; eauto.
-      econs; eauto. econs 2; eauto. econs; eauto.
-Qed.
-
-
-Lemma shorter_memory_write mem_src mem_tgt loc from1 to1 val released mem_tgt' from'
-      (SHORTER: shorter_memory mem_src mem_tgt)
-      (ADD: Memory.write Memory.bot mem_tgt loc from1 to1 val released Memory.bot mem_tgt' Memory.op_kind_add)
-      (TO: Time.le from1 from')
-      (FROM: Time.lt from' to1)
-  :
-    exists mem_src',
-      (<<ADD: Memory.write Memory.bot mem_src loc from' to1 val released Memory.bot mem_src' Memory.op_kind_add>>) /\  
-      (<<SHORTER: shorter_memory mem_src' mem_tgt'>>).  
-Proof.
-  dup SHORTER. inv SHORTER. inv ADD. inv PROMISE.
-  exploit write_succeed; eauto.
-  - instantiate (1:=mem_src). instantiate (1:=loc).
-    ii. eapply COVER in COVER0. inv COVER0.
-    dup MEM. eapply Memory.add_get0 in MEM. des. 
-    dup GET. eapply Memory.add_get1 in GET; eauto.
-    exploit Memory.get_disjoint.
-    + eapply GET.
-    + eapply GET1.
-    + i. des; clarify.
-      eapply x0; eauto. inv H. econs; ss; eauto.
-      eapply TimeFacts.le_lt_lt; eauto.
-  - inv MEM. inv ADD. inv MSG_WF. inv TS. eauto.
-  - inv MEM. inv ADD. eauto.
-  - i. des. inv WRITE. inv PROMISE. esplits; eauto. econs.
-    + i. erewrite Memory.add_o in GET; eauto.      
-      erewrite Memory.add_o; cycle 1; eauto. des_ifs; eauto.
-    + i. inv COV. erewrite Memory.add_o in GET; eauto. des_ifs.
-      * ss; des; clarify. eapply Memory.add_get0 in MEM. des.
-        econs; eauto. inv ITV. econs; eauto.
-        ss. eapply TimeFacts.le_lt_lt; eauto.
-      * exploit COVER.
-        { econs; eauto. }
-        intros COV. inv COV. eapply Memory.add_get1 in GET0; eauto.
-        econs; eauto.
-Qed
-
+    forget_statelocal (st, lc1) (st, lc2)
 .
 
-ThreadEvent.t  
-  Lemma write_succeed mem1 loc from1 to1 val released
-      (NCOVER: forall t (COVER: covered loc t mem1),
-          ~ Interval.mem (from1, to1) t)
-      (TO: Time.le (View.rlx (View.unwrap released) loc) to1)
-      (FROMTO: Time.lt from1 to1)
-      (MSGWF: Message.wf (Message.full val released))
-  :
-    exists mem2,
-      (<<WRITE: Memory.write Memory.bot mem1 loc from1 to1 val released Memory.bot mem2 Memory.op_kind_add>>).
-Proof.
-  exploit Memory.add_exists; eauto.
-  { instantiate (1:=mem1). instantiate (1:=loc).
-    ii. eapply NCOVER; eauto. econs; eauto. }
-  i. des. exists mem2.
-  exploit Memory.add_exists; eauto.
-  { instantiate (1:=Memory.bot). instantiate (1:=loc).
-    ii. rewrite Memory.bot_get in *. clarify. } i. des.
-  econs.
-  - econs; eauto; ss.
-  - exploit Memory.remove_exists; eauto.
-    { eapply Memory.add_get0 in x1. des. eauto. } i. des.
-    exploit MemoryFacts.MemoryFacts.add_remove_eq; eauto.
-    i. clarify.
-Qed.
-
-
-Lemma shorter_memory_write mem_src mem_tgt loc from to msg mem_tgt' from'
-      (SHORTER: shorter_memory mem_src mem_tgt)
-      (ADD: Memory.write mem_tgt loc from to msg mem_tgt')
-      (TO: Time.le from' from)
-      (FROM: Time.lt from' to)
-  :
-    exists mem_src',
-      (<<ADD: Memory.add mem_src loc from to msg mem_src'>>) /\  
-      (<<SHORTER: shorter_memory mem_src' mem_tgt'>>).  
-Proof.
-
-  
-
-
-  
-  
-  
-  
-Lemma shorter_memory_step
-      P lang th_src th_tgt th_tgt' st st' v v' prom prom' sc sc'
-      mem_tgt mem_tgt' mem_src e
-      (STEP: (@pred_step (P /1\ no_promise) lang) e th_tgt th_tgt')
-      (TH_SRC: th_src = Thread.mk lang st (Local.mk v prom) sc mem_src)
-      (TH_TGT0: th_tgt = Thread.mk lang st (Local.mk v prom) sc mem_tgt)
-      (TH_TGT1: th_tgt' = Thread.mk lang st' (Local.mk v' prom') sc' mem_tgt')
-      (SHORTER: shorter_memory mem_src mem_tgt)
-  :
-    exists mem_src',
-      (<<STEP: (@pred_step (P /1\ no_promise) lang)
-                 e th_src
-                 (Thread.mk lang st' (Local.mk v' prom') sc' mem_src')>>) /\
-      (<<SHORTER: shorter_memory mem_src' mem_tgt'>>).
-Proof.
-  dup SHORTER. inv SHORTER. inv STEP. inv STEP0. des. inv STEP.
-  - inv STEP0. ss.
-  - inv STEP0. inv LOCAL.
-    + exists mem_src; eauto. econs; eauto. econs; eauto.
-      
-
-
-    
-    inv LOCAL. ss. clarify.
-    esplits. econs; eauto. econs; eauto. econs 1; eauto. econs; eauto.
-  - inv STEP0. inv LOCAL; ss.
-    + esplits. econs; eauto. econs; eauto. econs 2; eauto. econs; eauto.
-    + esplits. econs; eauto. econs; eauto. econs 2; eauto. econs; eauto.
-    + inv LOCAL0. ss. clarify. exists sc_src. 
-      econs; eauto. econs; eauto. econs 2; eauto. econs; eauto.
-      econs; eauto. econs; eauto. ss.
-      inv WRITABLE. econs; eauto.
-    + inv LOCAL1. ss. inv LOCAL2. ss. clarify. exists sc_src. 
-      econs; eauto. econs; eauto. econs 2; eauto. econs; eauto.
-      econs; eauto. econs; eauto. ss.
-      inv WRITABLE. econs; eauto.
-    + inv LOCAL0. ss. clarify.
-      esplits. econs; eauto. econs; eauto. econs 2; eauto. econs; eauto.
-      econs; eauto. econs; eauto. ss. f_equal.
-      unfold TView.write_fence_tview. ss. des_ifs.
-Qed.
-
-
-Lemma not_attatched_write
-      L lang th_tgt th_tgt' st st' v v' prom prom' sc sc'
-      mem_tgt mem_tgt' e_tgt
-      (SCMAX: ~ promise_view_consistent prom sc)
-      (TH_TGT0: th_tgt = Thread.mk lang st (Local.mk v Memort.bot) sc mem_tgt)
-      (TH_TGT1: th_tgt' = Thread.mk lang st' (Local.mk v' prom') sc' mem_tgt')
-      (STEP: (@pred_step (no_update_on L) lang) e_tgt th_tgt th_tgt')
-  :
-    no_sc e_tgt.
-Proof.
-
-
-Lemma not_attatched_write
-      L lang th_tgt th_tgt' st st' v v' prom prom' sc sc'
-      mem_tgt mem_tgt' e_tgt
-      (SCMAX: ~ promise_view_consistent prom sc)
-      (TH_TGT0: th_tgt = Thread.mk lang st (Local.mk v Memort.bot) sc mem_tgt)
-      (TH_TGT1: th_tgt' = Thread.mk lang st' (Local.mk v' prom') sc' mem_tgt')
-      (STEP: (@pred_step (no_update_on L) lang) e_tgt th_tgt th_tgt')
-  :
-    no_sc e_tgt.
-Proof.
-      
-                         
-    Memory.
-    
-    (<<GET: exists msg, <<MSG: Memory.get l t = Some msg>> >>) /\
-    (<<NOATTATCH: exists msg,
-
-        
-
-                  Memory.adjacent
-  covered
-
-
-
-
-
-
-Lemma consistent_read_no_self_promise
-      lang th_tgt th_tgt' st st' v v' prom prom' sc sc'
-      mem_tgt mem_tgt' e_tgt
-      (LOCALWF: Local.wf (Local.mk v prom) mem_tgt)
-      (CLOSED: Memory.closed mem_tgt)
-      (SC: Memory.closed_timemap sc mem_tgt)
-      (TH_TGT0: th_tgt = Thread.mk lang st (Local.mk v prom) sc mem_tgt)
-      (TH_TGT1: th_tgt' = Thread.mk lang st' (Local.mk v' prom') sc' mem_tgt')
-      (CONSISTENT: local_consistent (Local.mk v' prom'))
-      (STEP: Thread.step_allpf e_tgt th_tgt th_tgt')
-  :
-    no_read_msgs prom.(promised) e_tgt.
-Proof.
-
-Lemma forget_exists prom mem_tgt:
-  exists mem_src, <<FORGET: Forget.forget_memory prom.(promised) mem_src mem_tgt>>.
-Proof.
-  hexploit (Memory.finite_sound_exists prom); eauto. i. des.
-  hexploit (forget_exists_list dom mem_tgt). i. des. exists mem_src.
-  inv FORGET. econs; i.
-  - eapply COMPLETE; eauto. ii. eapply NPROMS.
-    exploit H0; eauto. i. des. econs; eauto.
-  - eapply FORGET0; eauto. inv PROMS. destruct msg. eauto.
-Qed.
-
-
-Memory.get
-                                  
-  ex
-
-  
-  revert prom mem_tgt H. induction dom; ss.
-  - i. exists mem_tgt. econs; ss.
-    i. inv PROMS. destruct msg. exfalso. eauto.
-  - i. destruct a as [loc to].
-    exploit IHdom.
-
-    destruct (Memory.get loc to mem_src). 
-    
-    
-  
-  
-  
-      
-  
-  Inductive forget_memory P msrc mtgt : Prop :=
-  | forget_memory_intro
-      (* (FUTURE: Memory.le msrc mtgt) *)
-      (COMPLETE: forall l t (NPROMS: ~ P l t),
-          Memory.get l t msrc = Memory.get l t mtgt)
-      (FORGET: forall l t (PROMS: P l t), Memory.get l t msrc = None)
-  .
-
-    
-
-
-        Inductive forget_memory P msrc mtgt : Prop :=
-  | forget_memory_intro
-      (* (FUTURE: Memory.le msrc mtgt) *)
-      (COMPLETE: forall l t (NPROMS: ~ P l t),
-          Memory.get l t msrc = Memory.get l t mtgt)
-      (FORGET: forall l t (PROMS: P l t), Memory.get l t msrc = None)
-  .
-
-
-Memory.finite
-Lemma forget_step
-Configuration.step
-      
-
-Lemma unchanged_on_step
-      (
-      
-
-
-  
-Inductive unchanged_on (P: Loc.t -> Time.t -> Prop) m0 m1 : Prop :=
-| unchanged_on_intro
-    (NCOV: forall l t (IN: P l t) (COV: covered l t m1), covered l t m0)
-    (FUTURE : Memory.le m0 m1)
+Inductive full_promised (mem: Memory.t) (loc: Loc.t) (to: Time.t) : Prop :=
+| full_promised_intro
+    from val released
+    (GET: Memory.get loc to mem = Some (from, Message.full val released))
 .
 
+Inductive all_promises (c: Configuration.t) (P: IdentMap.key -> Prop)
+          (l: Loc.t) (t: Time.t) : Prop :=
+| all_promises_intro
+    tid st lc
+    (TID1: IdentMap.find tid c.(Configuration.threads) = Some (st, lc))
+    (PROMISED: promised lc.(Local.promises) l t)
+    (SAT: P tid)
+.
 
-Lemma pf_step_hold_other
-      c1_src c1_tgt
-      c3_tgt e tid mlast updates tf
-      (SIM: sim_pf mlast updates c1_src c1_tgt)
-      (STEP_TGT: Configuration.step e tid c1_tgt c3_tgt)
-  :
-    exists th2_src th3_src,
-      (<<STEPS_SRC: rtc (tau (@Thread.program_step _))
-                       (to_thread
-                          (Threads.find tid c1_src.(Configuration.threads))
-                          c1_src.(Configuration.sc)
-                          c1_src.(Configuration.memory))
-                       th2_src>>) /\
-      (<<STEP_SRC: opt_pftstep e th2_src th3_src>>) /\
-      (<<SC: th3_src.(Thread.sc) = c3_tgt.(Configuration.sc)>> /\
-            <<MEM: Forget.forget_memory
-                     (all_promises c3_tgt)
-                     th3_src.(Thread.memory) c3_tgt.(Configuration.memory)>>) /\
-      (<<ST: Forget.forget_state
-              (StateLocal.mk _ th3_src.(Thread.state) th3_src.(Thread.local))
-              (Threads.find tid c3_tgt.(Configuration.threads))>>) /\
-      (<<HOLD: forall tid2 (NEQ : tid <> tid2),
-                Inv.hold
-                  (Threads.find tid2 c1_src.(Configuration.threads))
-                  (Locked.t (c1_tgt.(Configuration.mpreds) tid2))
-                  ((Threads.find tid2 c3_tgt.(Configuration.threads)).(StateLocal.local).(Local.promises))
-                  (skylast tid2)
-                  (mlast tid2) th3_src.(Thread.memory)>>).
-Proof.
-Admitted.
+Inductive pf_sim_memory (proms: Loc.t -> Time.t -> Prop) (mem_src mem_tgt: Memory.t): Prop :=
+| pf_sim_memory_intro
+    mem_inter
+    (FORGET: forget_memory proms mem_inter mem_tgt)
+    (SHORTER: shorter_memory mem_src mem_inter) 
+.
 
-(* Lemma inv_monotone st proms sky updates mlast v0 v1 *)
-(*       (LE: TimeMap.le v0 v1) *)
-(*       (INV: Inv.t st proms sky updates mlast v1) *)
-(*   : *)
-(*     Inv.t st proms sky updates mlast v0. *)
-(* Proof. *)
-(*   inv INV. econs; i. *)
-(*   - eapply PROMS; ss. *)
-(*     inv FUTURE. econs; ss. *)
-(*     i. etrans; eauto. *)
-(*   - eapply UPDATE; ss. *)
-(*     inv FUTURE. econs; ss. *)
-(*     i. etrans; eauto. *)
-(* Qed. *)
+Inductive forget_config csrc ctgt : Prop :=
+| forget_configuration_intro
+    (THS : forall tid, option_rel
+                         forget_statelocal 
+                         (IdentMap.find tid csrc.(Configuration.threads))
+                         (IdentMap.find tid ctgt.(Configuration.threads)))
+    (SC : csrc.(Configuration.sc) = ctgt.(Configuration.sc))
+    (MEM : pf_sim_memory (all_promises ctgt (fun _ => True))
+                         (Configuration.memory csrc)
+                         (Configuration.memory ctgt))
+.
 
-(* Lemma inv_hold_self *)
-(*       st locked proms sky mem *)
-(*       (SKY: TimeMap.le (Memory.max_timemap mem) sky) *)
-(*       (PROM: forall l t, covered proms l t -> covered mem l t -> False) *)
-(*   : *)
-(*     Inv.hold st locked proms sky mem mem *)
-(* . *)
-(* Proof. *)
-(*   ii. econs; i; ss; eauto. *)
-(*   revert INV. induction FUTURE; ss; i.     *)
-(*   clarify. unfold TimeMap.add in *. ss. *)
-(*   des_ifs. *)
-(*   - left. eapply TimeFacts.le_lt_lt; cycle 1; eauto. *)
-(*     eapply IHFUTURE; ss. *)
-(*     eapply inv_monotone; eauto. *)
-(*     ii. des_ifs. *)
-(*     + left. eauto. *)
-(*     + right. ss. *)
-(*   - eapply IHFUTURE; eauto. *)
-(*     eapply inv_monotone; eauto. *)
-(*     ii. des_ifs. *)
-(*     + left. eauto. *)
-(*     + right. ss. *)
-(* Qed. *)
-
-(* (* TODO *) *)
-(* Lemma consistent_inhabited *)
-(*       mlast skylast c_src c_tgt tid *)
-(*       (FORGET: Forget.forget_config c_src c_tgt) *)
-(*       (RACEFREE: pf_racefree c_src) *)
-(*       (INHABITED: forall tid' (NEQ: tid'<>tid), *)
-(*           Inv.inhabited *)
-(*             (Threads.find tid' c_src.(Configuration.threads)) *)
-(*             (Locked.t (c_tgt.(Configuration.mpreds) tid')) *)
-(*             ((Threads.find tid' c_tgt.(Configuration.threads)).(StateLocal.local).(Local.promises)) *)
-(*             (skylast tid') (mlast tid')) *)
-(*       (HOLD: forall tid' (NEQ: tid'<>tid), *)
-(*           Inv.hold *)
-(*             (Threads.find tid' c_src.(Configuration.threads)) *)
-(*             (Locked.t (c_tgt.(Configuration.mpreds) tid')) *)
-(*             ((Threads.find tid' c_tgt.(Configuration.threads)).(StateLocal.local).(Local.promises)) *)
-(*             (skylast tid') (mlast tid') c_src.(Configuration.memory)) *)
-(*       (CONSISTENT: Thread.consistent *)
-(*                      (c_tgt.(Configuration.mpreds) tid) *)
-(*                      bot2 *)
-(*                      (to_thread *)
-(*                         (Threads.find tid c_tgt.(Configuration.threads)) *)
-(*                         (c_tgt.(Configuration.sc)) *)
-(*                         (c_tgt.(Configuration.memory)))) *)
-(*   : *)
-(*     Inv.inhabited *)
-(*       (Threads.find tid c_src.(Configuration.threads)) *)
-(*       (Locked.t (c_tgt.(Configuration.mpreds) tid)) *)
-(*       ((Threads.find tid c_tgt.(Configuration.threads)).(StateLocal.local).(Local.promises)) *)
-(*       (Memory.max_timemap c_tgt.(Configuration.memory)) c_src.(Configuration.memory). *)
-(* Admitted. *)
-
-
-(* Definition not_stuck lang (st: Language.state lang) := *)
-(*   exists st' e, Language.step _ e st st'. *)
-
-(* Lemma same_add_same ths tid st *)
-(*       (FIND: Threads.find tid ths = st) *)
-(*       (STEP: not_stuck _ st.(StateLocal.state)) *)
-(*   : *)
-(*     Threads.add tid st ths = ths. *)
-(* Proof. *)
-(*   eapply IdentMap.eq_leibniz. ii. *)
-(*   unfold Threads.find, Threads.add in *. *)
-(*   rewrite IdentMap.Facts.add_o. des_ifs. *)
-(*   exfalso. inv STEP. des. inv H. *)
-(* Qed. *)
-
-(* Ltac etatac := match goal with *)
-(*                  [|- ?x = ?y] => *)
-(*                  (try (destruct x; ss; clarify; eauto; fail));              *)
-(*                  (try (destruct y; ss; clarify; eauto; fail)); *)
-(*                  (try (dependent destruction x; ss; clarify; eauto; fail)); *)
-(*                  (try (dependent destruction y; ss; clarify; eauto; fail)) *)
-(*                end. *)
-
-
-(* Lemma sim_pf_step *)
-(*       c1_src c1_tgt *)
-(*       c3_tgt e tid tf *)
-(*       (SIM: sim_pf_all c1_src c1_tgt) *)
-(*       (STEP_TGT: Configuration.step tf e tid c1_tgt c3_tgt) *)
-(*   : *)
-(*     exists c3_src, *)
-(*       (<<STEP_SRC: opt pftstep e tid c1_src c3_src>>) /\ *)
-(*       (<<SIM: sim_pf_all c3_src c3_tgt>>) *)
-(* . *)
-(* Proof. *)
-(*   assert (NOABORT: e <> Some MachineEvent.abort). *)
-(*   { eapply no_abort; eauto. } *)
-(*   inv SIM. exploit pf_step_hold_other; eauto. *)
-(*   inv SIM0. i. des. *)
-
-(*   assert (SIMPF: sim_pf_all *)
-(*                    (Configuration.mk *)
-(*                       (Threads.add tid (StateLocal.mk _ (th3_src.(Thread.state)) *)
-(*                                                       (th3_src.(Thread.local)))  *)
-(*                                    (Configuration.threads c1_src)) *)
-(*                       (Configuration.sc c3_tgt) *)
-(*                       th3_src.(Thread.memory) MPreds.init) *)
-(*                    c3_tgt). *)
-
-(*   { *)
-(*       destruct th3_src. econs. *)
-(*       instantiate (1:= fun tid' => if (Ident.eq_dec tid tid') then Memory.max_timemap c3_tgt.(Configuration.memory) else skylast tid'). *)
-(*       instantiate (1:= fun tid' => if (Ident.eq_dec tid tid') then memory else mlast tid'). *)
-(*       assert (RACEFREE0: pf_racefree *)
-(*     {| *)
-(*     Configuration.threads := Threads.add tid *)
-(*                                {| *)
-(*                                StateLocal.lang := StateLocal.lang *)
-(*                                                 (Threads.find tid *)
-(*                                                 (Configuration.threads *)
-(*                                                 c1_src)); *)
-(*                                StateLocal.state := state; *)
-(*                                StateLocal.local := local |} *)
-(*                                (Configuration.threads c1_src); *)
-(*     Configuration.sc := sc; *)
-(*     Configuration.memory := memory; *)
-(*     Configuration.mpreds := MPreds.init |}). *)
-(*       { eapply pf_racefree_step; eauto. ss. clarify. *)
-(*         admit. *)
-(*         (* inv STEPS_SRC0. *) *)
-(*         (* econs; [|left]. econs. econs. econs; ss; eauto. *) *)
-(*         (* etatac. *) *)
-(*       } *)
-(*       econs; ss; clarify; eauto. *)
-(*       * econs; i; ss. *)
-(*         inv FORGET. addtac. *)
-(*         inv STEP_TGT; ss; addtac. *)
-(*       * i. des_ifs; addtac. *)
-(*         -- Opaque Inv.inhabited. *)
-(*           set *)
-(*              (C:= @consistent_inhabited *)
-(*                 (fun tid' => if (Ident.eq_dec tid0 tid') then memory else mlast tid') *)
-(*                 (fun tid' => if (Ident.eq_dec tid0 tid') then Memory.max_timemap c3_tgt.(Configuration.memory) else skylast tid') *)
-(*                 (Configuration.mk *)
-(*                    (Threads.add tid0 (StateLocal.mk _ state local)  *)
-(*                                 (Configuration.threads c1_src)) *)
-(*                    (Configuration.sc c3_tgt) memory MPreds.init) *)
-(*                 c3_tgt tid0); ss; i; eauto. *)
-(*           addtac. *)
-(*           eapply C; eauto; clear C. *)
-(*            ++ inv FORGET. econs; i; ss; addtac. *)
-(*               replace (Threads.find tid (Configuration.threads c3_tgt)) with *)
-(*                   (Threads.find tid (Configuration.threads c1_tgt)); eauto. *)
-(*               inv STEP_TGT; addtac; addtac. *)
-(*            ++ i. addtac. ss. *)
-(*               replace (Locked.t (Configuration.mpreds c3_tgt tid')) with *)
-(*                   (Locked.t (Configuration.mpreds c1_tgt tid')); cycle 1. *)
-(*               { inv STEP_TGT; repeat addtac. } *)
-(*               replace (Threads.find tid' (Configuration.threads c3_tgt)) with *)
-(*                   (Threads.find tid' (Configuration.threads c1_tgt)); eauto. *)
-(*               { inv STEP_TGT; repeat addtac. } *)
-(*            ++ i. addtac. *)
-(*               replace (Locked.t (Configuration.mpreds c3_tgt tid')) with *)
-(*                   (Locked.t (Configuration.mpreds c1_tgt tid')); eauto. *)
-(*               { inv STEP_TGT; repeat addtac. } *)
-(*            ++ inv STEP_TGT; repeat addtac; unfold to_thread; ss; eauto. *)
-(*               ** eapply Thread.consistent_le; eauto. clarify. *)
-(*               ** destruct (Threads.find tid0 (Configuration.threads c1_tgt)). *)
-(*                  dependent destruction TID. ss. *)
-(*                  eapply Thread.consistent_le; eauto. clarify. *)
-
-(*         -- replace (Locked.t (Configuration.mpreds c3_tgt tid0)) with *)
-(*                   (Locked.t (Configuration.mpreds c1_tgt tid0)); cycle 1. *)
-(*            { inv STEP_TGT; repeat addtac. } *)
-(*            replace (Threads.find tid0 (Configuration.threads c3_tgt)) with *)
-(*                (Threads.find tid0 (Configuration.threads c1_tgt)); eauto. *)
-(*            { inv STEP_TGT; repeat addtac. } *)
-(*       * i. addtac. *)
-(*         -- eapply inv_hold_self. *)
-(*            ++ clear - MEM. admit. *)
-(*            ++ clear - MEM. i. inv MEM. *)
-(*               exploit FORGET; eauto. *)
-(*               econs. eauto. *)
-(*         -- replace (Locked.t (Configuration.mpreds c3_tgt tid0)) with *)
-(*                   (Locked.t (Configuration.mpreds c1_tgt tid0)); eauto. *)
-(*            { inv STEP_TGT; repeat addtac. } *)
-(*       * eapply finite_hole_preserve; eauto. *)
-(*       * i. clarify. des_ifs. rewrite <- UNCHANGED. *)
-(*         { inv STEP_TGT; eauto; ss. *)
-(*           inv RELY. addtac. *)
-(*           specialize (WRITABLE l). des; eauto. *)
-(*           exfalso. dup LK. *)
-(*           inv LK; destruct hd; *)
-(*             specialize (WRITABLE tid0 t t0 tl n0 (eq_sym H0)); *)
-(*             rewrite <- H0 in *; *)
-(*             eapply Locked.locked_non_writable; eauto. *)
-(*         } *)
-(*         inv STEP_TGT; eauto; addtac; ss; des_ifs. *)
-(*       * eapply Configuration.step_future; eauto. *)
-(*       * eapply Configuration.step_future; eauto. *)
-(*       * eapply Configuration.step_future; eauto. *)
-(*     } *)
+Module Inv.
   
-(*   eapply rtc_tail in STEPS_SRC. des. des; inv STEP_SRC. *)
-(*   - exists (Configuration.mk *)
-(*                    (Threads.add tid (StateLocal.mk _ (th3_src.(Thread.state)) *)
-(*                                                     (th3_src.(Thread.local)))  *)
-(*                                 (Configuration.threads c1_src)) *)
-(*                    (Configuration.sc c3_tgt) *)
-(*                    th3_src.(Thread.memory) MPreds.init). *)
-(*     split. *)
-(*     + inv STEPS_SRC0. rewrite <- EVENT. *)
-(*       right. *)
-(*       destruct (Threads.find tid (Configuration.threads c1_src)) eqn: TEQ. *)
-(*       econs; ss; eauto. *)
-(*       destruct th3_src. rewrite <- SC. ss. *)
+  Inductive t lang (st: Language.state lang) lc
+            (proms: Memory.t) (updates : Loc.t -> Time.t -> Prop) (mlast: Memory.t): Prop :=
+  | inv_intro
+      (PROMS: forall
+          loc to m sc (PROM : full_promised proms loc to)
+          (FUTURE: unchanged_on
+                     (fun loc to => covered loc to proms)
+                     mlast m)
+          (UNCHANGED: not_attatched updates m),          
+          exists st' lc' sc' m',
+            (<<STEPS : rtc (tau (@Thread.program_step _))
+                           (Thread.mk _ st lc sc m)
+                           (Thread.mk _ st' lc' sc' m')>>) /\
+            (<<WRITING : is_writing _ st' loc Ordering.relaxed>>))
+      (UPDATE : forall
+          loc to m sc (UPD : updates loc to)
+          (FUTURE: unchanged_on
+                     (fun loc to => covered loc to proms)
+                     mlast m)
+          (UNCHANGED: not_attatched updates m),
+          exists st' lc' sc' m',
+            (<<STEPS : rtc (tau (@Thread.program_step _))
+                           (Thread.mk _ st lc sc m)
+                           (Thread.mk _ st' lc' sc' m')>>) /\
+            (<<READING : is_updating _ st' loc Ordering.relaxed>>)
+      )
+  .
 
-(*     +  *)
-(*     { *)
-(*       destruct th3_src. econs. *)
-(*       instantiate (1:= fun tid' => if (Ident.eq_dec tid tid') then Memory.max_timemap c3_tgt.(Configuration.memory) else skylast tid'). *)
-(*       instantiate (1:= fun tid' => if (Ident.eq_dec tid tid') then memory else mlast tid'). *)
-(*       assert (RACEFREE0: pf_racefree *)
-(*     {| *)
-(*     Configuration.threads := Threads.add tid *)
-(*                                {| *)
-(*                                StateLocal.lang := StateLocal.lang *)
-(*                                                 (Threads.find tid *)
-(*                                                 (Configuration.threads *)
-(*                                                 c1_src)); *)
-(*                                StateLocal.state := state; *)
-(*                                StateLocal.local := local |} *)
-(*                                (Configuration.threads c1_src); *)
-(*     Configuration.sc := sc; *)
-(*     Configuration.memory := memory; *)
-(*     Configuration.mpreds := MPreds.init |}). *)
-(*       { eapply pf_racefree_step; eauto. ss. clarify. *)
-(*         inv STEPS_SRC0. *)
-(*         econs; [|left]. econs. econs. econs; ss; eauto. *)
-(*         etatac. } *)
-(*       econs; ss; clarify; eauto. *)
-(*       * econs; i; ss. *)
-(*         inv FORGET. addtac. *)
-(*         inv STEP_TGT; ss; addtac. *)
-(*       * i. des_ifs; addtac. *)
-(*         -- Opaque Inv.inhabited. *)
-(*           set *)
-(*              (C:= @consistent_inhabited *)
-(*                 (fun tid' => if (Ident.eq_dec tid0 tid') then memory else mlast tid') *)
-(*                 (fun tid' => if (Ident.eq_dec tid0 tid') then Memory.max_timemap c3_tgt.(Configuration.memory) else skylast tid') *)
-(*                 (Configuration.mk *)
-(*                    (Threads.add tid0 (StateLocal.mk _ state local)  *)
-(*                                 (Configuration.threads c1_src)) *)
-(*                    (Configuration.sc c3_tgt) memory MPreds.init) *)
-(*                 c3_tgt tid0); ss; i; eauto. *)
-(*           addtac. *)
-(*           eapply C; eauto; clear C. *)
-(*            ++ inv FORGET. econs; i; ss; addtac. *)
-(*               replace (Threads.find tid (Configuration.threads c3_tgt)) with *)
-(*                   (Threads.find tid (Configuration.threads c1_tgt)); eauto. *)
-(*               inv STEP_TGT; addtac; addtac. *)
-(*            ++ i. addtac. ss. *)
-(*               replace (Locked.t (Configuration.mpreds c3_tgt tid')) with *)
-(*                   (Locked.t (Configuration.mpreds c1_tgt tid')); cycle 1. *)
-(*               { inv STEP_TGT; repeat addtac. } *)
-(*               replace (Threads.find tid' (Configuration.threads c3_tgt)) with *)
-(*                   (Threads.find tid' (Configuration.threads c1_tgt)); eauto. *)
-(*               { inv STEP_TGT; repeat addtac. } *)
-(*            ++ i. addtac. *)
-(*               replace (Locked.t (Configuration.mpreds c3_tgt tid')) with *)
-(*                   (Locked.t (Configuration.mpreds c1_tgt tid')); eauto. *)
-(*               { inv STEP_TGT; repeat addtac. } *)
-(*            ++ inv STEP_TGT; repeat addtac; unfold to_thread; ss; eauto. *)
-(*               ** eapply Thread.consistent_le; eauto. clarify. *)
-(*               ** destruct (Threads.find tid0 (Configuration.threads c1_tgt)). *)
-(*                  dependent destruction TID. ss. *)
-(*                  eapply Thread.consistent_le; eauto. clarify. *)
-
-(*         -- replace (Locked.t (Configuration.mpreds c3_tgt tid0)) with *)
-(*                   (Locked.t (Configuration.mpreds c1_tgt tid0)); cycle 1. *)
-(*            { inv STEP_TGT; repeat addtac. } *)
-(*            replace (Threads.find tid0 (Configuration.threads c3_tgt)) with *)
-(*                (Threads.find tid0 (Configuration.threads c1_tgt)); eauto. *)
-(*            { inv STEP_TGT; repeat addtac. } *)
-(*       * i. addtac. *)
-(*         -- eapply inv_hold_self. *)
-(*            ++ clear - MEM. admit. *)
-(*            ++ clear - MEM. i. inv MEM. *)
-(*               exploit FORGET; eauto. *)
-(*               econs. eauto. *)
-(*         -- replace (Locked.t (Configuration.mpreds c3_tgt tid0)) with *)
-(*                   (Locked.t (Configuration.mpreds c1_tgt tid0)); eauto. *)
-(*            { inv STEP_TGT; repeat addtac. } *)
-(*       * eapply finite_hole_preserve; eauto. *)
-(*       * i. clarify. des_ifs. rewrite <- UNCHANGED. *)
-(*         { inv STEP_TGT; eauto; ss. *)
-(*           inv RELY. addtac. *)
-(*           specialize (WRITABLE l). des; eauto. *)
-(*           exfalso. dup LK. *)
-(*           inv LK; destruct hd; *)
-(*             specialize (WRITABLE tid0 t t0 tl n0 (eq_sym H0)); *)
-(*             rewrite <- H0 in *; *)
-(*             eapply Locked.locked_non_writable; eauto. *)
-(*         } *)
-(*         inv STEP_TGT; eauto; addtac; ss; des_ifs. *)
-(*       * eapply Configuration.step_future; eauto. *)
-(*       * eapply Configuration.step_future; eauto. *)
-(*       * eapply Configuration.step_future; eauto. *)
-(*     } *)
-(*   -  *)
-(* Admitted. *)
+End Inv.
 
 
+Inductive sim_pf
+          (mlast: Ident.t -> Memory.t) (updates: Ident.t -> (Loc.t -> Time.t -> Prop))
+          (c_src c_tgt: Configuration.t) : Prop :=
+| sim_pf_intro
+    (FORGET: forget_config c_src c_tgt)
+    (RACEFREE: pf_racefree c_src)
+    (INV:
+       forall
+         tid lang_src st_src lc_src lang_tgt st_tgt lc_tgt
+         (TIDSRC: IdentMap.find tid c_src.(Configuration.threads) =
+                  Some (existT _ lang_src st_src, lc_src))
+         (TIDTGT: IdentMap.find tid c_tgt.(Configuration.threads) =
+                  Some (existT _ lang_tgt st_tgt, lc_tgt)),
+         Inv.t _ st_src lc_src lc_tgt.(Local.promises) (updates tid) (mlast tid))
+    (FUTURE:
+       forall tid lang_src st_src lc_src
+              (TIDSRC: IdentMap.find tid c_src.(Configuration.threads) =
+                       Some (existT _ lang_src st_src, lc_src)),
+         unchanged_on
+           (fun loc to => covered loc to lc_src.(Local.promises))
+           (mlast tid) c_src.(Configuration.memory))
+    (NOATTATCH:
+       forall tid,
+         not_attatched (updates tid) c_src.(Configuration.memory))
+    (WFSRC: Configuration.wf c_src)
+    (WFTGT: Configuration.wf c_tgt)
+.
 
+Inductive sim_pf_all c_src c_tgt: Prop :=
+| sim_pf_all_intro mlast updates (SIM : sim_pf mlast updates c_src c_tgt)
+.
 
-
-
-
-(* Lemma sim_pf_step *)
-(*       c1_src c1_tgt *)
-(*       c3_tgt e tid tf mlast skylast *)
-(*       (SIM: sim_pf c1_src c1_tgt mlast skylast) *)
-(*       (STEP_TGT: Configuration.step tf e tid c1_tgt c3_tgt) *)
-(*   : *)
-(*     exists c3_src, *)
-(*       (<<STEP_SRC: opt pftstep e tid c1_src c3_src>>) /\ *)
-(*       (<<SIM: sim_pf *)
-(*                 c3_src c3_tgt *)
-(*                 (fun tid' => if (Ident.eq_dec tid tid') then c3_src.(Configuration.memory) else skylast tid') *)
-(*                 (fun tid' => if (Ident.eq_dec tid tid') then Memory.max_timemap c3_tgt.(Configuration.memory) else skylast tid') *)
-
-                
-(* (fun tid' => if (Ident.eq_dec tid tid') then Memory.max_timemap c3_tgt.(Configuration.memory) else skylast tid') *)
-                         
-(*                          >>) *)
-(* . *)
-(* Proof. *)
-(*   assert (NOABORT: e <> Some MachineEvent.abort). *)
-(*   { eapply no_abort; eauto. } *)
-(*   inv SIM. exploit pf_step_hold_other; eauto. *)
-(*   inv SIM0. i. des. *)
-(*   eapply rtc_tail in STEPS_SRC. des; inv STEP_SRC. *)
-(*   - exists (Configuration.mk *)
-(*                    (Threads.add tid (StateLocal.mk _ (th3_src.(Thread.state)) *)
-(*                                                     (th3_src.(Thread.local)))  *)
-(*                                 (Configuration.threads c1_src)) *)
-(*                    (Configuration.sc c3_tgt) *)
-(*                    th3_src.(Thread.memory) MPreds.init). *)
-(*     split. *)
-(*     + inv STEPS_SRC0. rewrite <- EVENT. *)
-(*       right. *)
-(*       destruct (Threads.find tid (Configuration.threads c1_src)) eqn: TEQ. *)
-(*       econs; ss; eauto. *)
-(*       destruct th3_src. rewrite <- SC. ss. *)
-
-(*     +  *)
-(*     { *)
-(*       destruct th3_src. econs. *)
-(*       instantiate (1:= fun tid' => if (Ident.eq_dec tid tid') then Memory.max_timemap c3_tgt.(Configuration.memory) else skylast tid'). *)
-(*       instantiate (1:= fun tid' => if (Ident.eq_dec tid tid') then memory else mlast tid'). *)
-(*       assert (RACEFREE0: pf_racefree *)
-(*     {| *)
-(*     Configuration.threads := Threads.add tid *)
-(*                                {| *)
-(*                                StateLocal.lang := StateLocal.lang *)
-(*                                                 (Threads.find tid *)
-(*                                                 (Configuration.threads *)
-(*                                                 c1_src)); *)
-(*                                StateLocal.state := state; *)
-(*                                StateLocal.local := local |} *)
-(*                                (Configuration.threads c1_src); *)
-(*     Configuration.sc := sc; *)
-(*     Configuration.memory := memory; *)
-(*     Configuration.mpreds := MPreds.init |}). *)
-(*       { eapply pf_racefree_step; eauto. ss. clarify. *)
-(*         inv STEPS_SRC0. *)
-(*         econs; [|left]. econs. econs. econs; ss; eauto. *)
-(*         etatac. } *)
-(*       econs; ss; clarify; eauto. *)
-(*       * econs; i; ss. *)
-(*         inv FORGET. addtac. *)
-(*         inv STEP_TGT; ss; addtac. *)
-(*       * i. des_ifs; addtac. *)
-(*         -- Opaque Inv.inhabited. *)
-(*           set *)
-(*              (C:= @consistent_inhabited *)
-(*                 (fun tid' => if (Ident.eq_dec tid0 tid') then memory else mlast tid') *)
-(*                 (fun tid' => if (Ident.eq_dec tid0 tid') then Memory.max_timemap c3_tgt.(Configuration.memory) else skylast tid') *)
-(*                 (Configuration.mk *)
-(*                    (Threads.add tid0 (StateLocal.mk _ state local)  *)
-(*                                 (Configuration.threads c1_src)) *)
-(*                    (Configuration.sc c3_tgt) memory MPreds.init) *)
-(*                 c3_tgt tid0); ss; i; eauto. *)
-(*           addtac. *)
-(*           eapply C; eauto; clear C. *)
-(*            ++ inv FORGET. econs; i; ss; addtac. *)
-(*               replace (Threads.find tid (Configuration.threads c3_tgt)) with *)
-(*                   (Threads.find tid (Configuration.threads c1_tgt)); eauto. *)
-(*               inv STEP_TGT; addtac; addtac. *)
-(*            ++ i. addtac. ss. *)
-(*               replace (Locked.t (Configuration.mpreds c3_tgt tid')) with *)
-(*                   (Locked.t (Configuration.mpreds c1_tgt tid')); cycle 1. *)
-(*               { inv STEP_TGT; repeat addtac. } *)
-(*               replace (Threads.find tid' (Configuration.threads c3_tgt)) with *)
-(*                   (Threads.find tid' (Configuration.threads c1_tgt)); eauto. *)
-(*               { inv STEP_TGT; repeat addtac. } *)
-(*            ++ i. addtac. *)
-(*               replace (Locked.t (Configuration.mpreds c3_tgt tid')) with *)
-(*                   (Locked.t (Configuration.mpreds c1_tgt tid')); eauto. *)
-(*               { inv STEP_TGT; repeat addtac. } *)
-(*            ++ inv STEP_TGT; repeat addtac; unfold to_thread; ss; eauto. *)
-(*               ** eapply Thread.consistent_le; eauto. clarify. *)
-(*               ** destruct (Threads.find tid0 (Configuration.threads c1_tgt)). *)
-(*                  dependent destruction TID. ss. *)
-(*                  eapply Thread.consistent_le; eauto. clarify. *)
-
-(*         -- replace (Locked.t (Configuration.mpreds c3_tgt tid0)) with *)
-(*                   (Locked.t (Configuration.mpreds c1_tgt tid0)); cycle 1. *)
-(*            { inv STEP_TGT; repeat addtac. } *)
-(*            replace (Threads.find tid0 (Configuration.threads c3_tgt)) with *)
-(*                (Threads.find tid0 (Configuration.threads c1_tgt)); eauto. *)
-(*            { inv STEP_TGT; repeat addtac. } *)
-(*       * i. addtac. *)
-(*         -- eapply inv_hold_self. *)
-(*            ++ clear - MEM. admit. *)
-(*            ++ clear - MEM. i. inv MEM. *)
-(*               exploit FORGET; eauto. *)
-(*               econs. eauto. *)
-(*         -- replace (Locked.t (Configuration.mpreds c3_tgt tid0)) with *)
-(*                   (Locked.t (Configuration.mpreds c1_tgt tid0)); eauto. *)
-(*            { inv STEP_TGT; repeat addtac. } *)
-(*       * eapply finite_hole_preserve; eauto. *)
-(*       * i. clarify. des_ifs. rewrite <- UNCHANGED. *)
-(*         { inv STEP_TGT; eauto; ss. *)
-(*           inv RELY. addtac. *)
-(*           specialize (WRITABLE l). des; eauto. *)
-(*           exfalso. dup LK. *)
-(*           inv LK; destruct hd; *)
-(*             specialize (WRITABLE tid0 t t0 tl n0 (eq_sym H0)); *)
-(*             rewrite <- H0 in *; *)
-(*             eapply Locked.locked_non_writable; eauto. *)
-(*         } *)
-(*         inv STEP_TGT; eauto; addtac; ss; des_ifs. *)
-(*       * eapply Configuration.step_future; eauto. *)
-(*       * eapply Configuration.step_future; eauto. *)
-(*       * eapply Configuration.step_future; eauto. *)
-(*     } *)
-(*   -  *)
-(* Admitted. *)
-
-
-(* Lemma sim_pf_step *)
-(*       c1_src c1_tgt *)
-(*       c3_tgt e tid tf *)
-(*       (SIM: sim_pf_all c1_src c1_tgt) *)
-(*       (STEP_TGT: Configuration.step tf e tid c1_tgt c3_tgt) *)
-(*   : *)
-(*     exists c3_src, *)
-(*       (<<STEP_SRC: opt pftstep e tid c1_src c3_src>>) /\ *)
-(*       (<<SIM: sim_pf_all c3_src c3_tgt>>) *)
-(* . *)
-(* Proof. *)
-(*   assert (NOABORT: e <> Some MachineEvent.abort). *)
-(*   { eapply no_abort; eauto. } *)
-(*   inv SIM. exploit pf_step_hold_other; eauto. *)
-(*   inv SIM0. i. des. *)
-(*   eapply rtc_tail in STEPS_SRC. des; inv STEP_SRC. *)
-(*   - exists (Configuration.mk *)
-(*                    (Threads.add tid (StateLocal.mk _ (th3_src.(Thread.state)) *)
-(*                                                     (th3_src.(Thread.local)))  *)
-(*                                 (Configuration.threads c1_src)) *)
-(*                    (Configuration.sc c3_tgt) *)
-(*                    th3_src.(Thread.memory) MPreds.init). *)
-(*     split. *)
-(*     + inv STEPS_SRC0. rewrite <- EVENT. *)
-(*       right. *)
-(*       destruct (Threads.find tid (Configuration.threads c1_src)) eqn: TEQ. *)
-(*       econs; ss; eauto. *)
-(*       destruct th3_src. rewrite <- SC. ss. *)
-
-(*     +  *)
-(*     { *)
-(*       destruct th3_src. econs. *)
-(*       instantiate (1:= fun tid' => if (Ident.eq_dec tid tid') then Memory.max_timemap c3_tgt.(Configuration.memory) else skylast tid'). *)
-(*       instantiate (1:= fun tid' => if (Ident.eq_dec tid tid') then memory else mlast tid'). *)
-(*       assert (RACEFREE0: pf_racefree *)
-(*     {| *)
-(*     Configuration.threads := Threads.add tid *)
-(*                                {| *)
-(*                                StateLocal.lang := StateLocal.lang *)
-(*                                                 (Threads.find tid *)
-(*                                                 (Configuration.threads *)
-(*                                                 c1_src)); *)
-(*                                StateLocal.state := state; *)
-(*                                StateLocal.local := local |} *)
-(*                                (Configuration.threads c1_src); *)
-(*     Configuration.sc := sc; *)
-(*     Configuration.memory := memory; *)
-(*     Configuration.mpreds := MPreds.init |}). *)
-(*       { eapply pf_racefree_step; eauto. ss. clarify. *)
-(*         inv STEPS_SRC0. *)
-(*         econs; [|left]. econs. econs. econs; ss; eauto. *)
-(*         etatac. } *)
-(*       econs; ss; clarify; eauto. *)
-(*       * econs; i; ss. *)
-(*         inv FORGET. addtac. *)
-(*         inv STEP_TGT; ss; addtac. *)
-(*       * i. des_ifs; addtac. *)
-(*         -- Opaque Inv.inhabited. *)
-(*           set *)
-(*              (C:= @consistent_inhabited *)
-(*                 (fun tid' => if (Ident.eq_dec tid0 tid') then memory else mlast tid') *)
-(*                 (fun tid' => if (Ident.eq_dec tid0 tid') then Memory.max_timemap c3_tgt.(Configuration.memory) else skylast tid') *)
-(*                 (Configuration.mk *)
-(*                    (Threads.add tid0 (StateLocal.mk _ state local)  *)
-(*                                 (Configuration.threads c1_src)) *)
-(*                    (Configuration.sc c3_tgt) memory MPreds.init) *)
-(*                 c3_tgt tid0); ss; i; eauto. *)
-(*           addtac. *)
-(*           eapply C; eauto; clear C. *)
-(*            ++ inv FORGET. econs; i; ss; addtac. *)
-(*               replace (Threads.find tid (Configuration.threads c3_tgt)) with *)
-(*                   (Threads.find tid (Configuration.threads c1_tgt)); eauto. *)
-(*               inv STEP_TGT; addtac; addtac. *)
-(*            ++ i. addtac. ss. *)
-(*               replace (Locked.t (Configuration.mpreds c3_tgt tid')) with *)
-(*                   (Locked.t (Configuration.mpreds c1_tgt tid')); cycle 1. *)
-(*               { inv STEP_TGT; repeat addtac. } *)
-(*               replace (Threads.find tid' (Configuration.threads c3_tgt)) with *)
-(*                   (Threads.find tid' (Configuration.threads c1_tgt)); eauto. *)
-(*               { inv STEP_TGT; repeat addtac. } *)
-(*            ++ i. addtac. *)
-(*               replace (Locked.t (Configuration.mpreds c3_tgt tid')) with *)
-(*                   (Locked.t (Configuration.mpreds c1_tgt tid')); eauto. *)
-(*               { inv STEP_TGT; repeat addtac. } *)
-(*            ++ inv STEP_TGT; repeat addtac; unfold to_thread; ss; eauto. *)
-(*               ** eapply Thread.consistent_le; eauto. clarify. *)
-(*               ** destruct (Threads.find tid0 (Configuration.threads c1_tgt)). *)
-(*                  dependent destruction TID. ss. *)
-(*                  eapply Thread.consistent_le; eauto. clarify. *)
-
-(*         -- replace (Locked.t (Configuration.mpreds c3_tgt tid0)) with *)
-(*                   (Locked.t (Configuration.mpreds c1_tgt tid0)); cycle 1. *)
-(*            { inv STEP_TGT; repeat addtac. } *)
-(*            replace (Threads.find tid0 (Configuration.threads c3_tgt)) with *)
-(*                (Threads.find tid0 (Configuration.threads c1_tgt)); eauto. *)
-(*            { inv STEP_TGT; repeat addtac. } *)
-(*       * i. addtac. *)
-(*         -- eapply inv_hold_self. *)
-(*            ++ clear - MEM. admit. *)
-(*            ++ clear - MEM. i. inv MEM. *)
-(*               exploit FORGET; eauto. *)
-(*               econs. eauto. *)
-(*         -- replace (Locked.t (Configuration.mpreds c3_tgt tid0)) with *)
-(*                   (Locked.t (Configuration.mpreds c1_tgt tid0)); eauto. *)
-(*            { inv STEP_TGT; repeat addtac. } *)
-(*       * eapply finite_hole_preserve; eauto. *)
-(*       * i. clarify. des_ifs. rewrite <- UNCHANGED. *)
-(*         { inv STEP_TGT; eauto; ss. *)
-(*           inv RELY. addtac. *)
-(*           specialize (WRITABLE l). des; eauto. *)
-(*           exfalso. dup LK. *)
-(*           inv LK; destruct hd; *)
-(*             specialize (WRITABLE tid0 t t0 tl n0 (eq_sym H0)); *)
-(*             rewrite <- H0 in *; *)
-(*             eapply Locked.locked_non_writable; eauto. *)
-(*         } *)
-(*         inv STEP_TGT; eauto; addtac; ss; des_ifs. *)
-(*       * eapply Configuration.step_future; eauto. *)
-(*       * eapply Configuration.step_future; eauto. *)
-(*       * eapply Configuration.step_future; eauto. *)
-(*     } *)
-(*   -  *)
-(* Admitted. *)
-
-
-
-
-
-
-(* Lemma self_promise_remove *)
-(*       P th_src th_tgt lang st v prom sc mem_src mem_tgt *)
-(*       (TH_SRC: th_src = to_thread Thread.mk lang st (Local.mk v Memory.bot) sc mem_src) *)
-(*       (TH_TGT: th_tgt = Thread.mk lang st (Local.mk v prom) sc mem_tgt) *)
-(*       (MEM: Forget.forget_memory (covered prom) mem_src mem_tgt) *)
-(*       (STEP: pred_step P lang e th_tgt th_tgt') *)
-(*   : *)
-(*     exists th_src', *)
-(*       (<<STEP: opt (pred_step P lang) e th_src th_src'>>) /\ *)
-(*       (<<MEM: Forget.forget_memory (covered opt (pred_step P lang) e th_src th_src'>>) /\ *)
-(*       (<<STEP: opt (pred_step P lang) e th_src th_src'>>) *)
-
-(* Lemma self_promise_remove *)
-(*       P th_src th_tgt lang st v prom sc mem_src mem_tgt *)
-(*       (TH_SRC: th_src = Thread.mk lang st (Local.mk v Memory.bot) sc mem_src) *)
-(*       (TH_TGT: th_tgt = Thread.mk lang st (Local.mk v prom) sc mem_tgt) *)
-(*       (MEM: Forget.forget_memory (covered prom) mem_src mem_tgt) *)
-(*       (STEP: pred_step P lang e th_tgt th_tgt') *)
-(*   : *)
-(*     exists th_src', *)
-(*       (<<STEP: opt (pred_step P lang) e th_src th_src'>>) /\ *)
-(*       (<<MEM: Forget.forget_memory (covered opt (pred_step P lang) e th_src th_src'>>) /\ *)
-(*       (<<STEP: opt (pred_step P lang) e th_src th_src'>>) *)
-      
-      
-(*       Thread.step Thread.t st lc sc mem1  *)
-
-(*       Thread.t *)
-(*       Thread.step *)
-(* Configuration.step *)
-
-(* opt (Thread.step *)
-
-
-(* Lemma sim_pf_sim_whole: *)
-(*   sim_pf_all <2= (sim_whole (fun _ => pftstep) Configuration.step). *)
-(* Proof. *)
-(*   pcofix CIH. ii. *)
-(*   pfold. econs. *)
-(*   - esplits; eauto. *)
-(*     inv PR. inv SIM. inv FORGET. *)
-(*     ii. specialize (THS tid). inv THS. *)
-(*     rewrite FIND in *. ss. econs; eauto. *)
-(*     specialize (TERMINAL_TGT tid). *)
-(*     destruct (Threads.find tid (Configuration.threads x1)). ss. *)
-(*     dependent destruction STATE. eapply TERMINAL_TGT; eauto. *)
-(*   - i. exploit sim_pf_step; eauto. i. des. esplits; eauto. *)
-(* Qed. *)
-
-(* Theorem drf_pf *)
-(*       s *)
-(*       (RACEFREE: pf_racefree (Configuration.init s)) *)
-(*   : *)
-(*     behaviors Configuration.step (Configuration.init s) <1= *)
-(*     behaviors (fun _ => pftstep) (Configuration.init s) *)
-(* . *)
-(* Proof. *)
-(*   apply sim_whole_adequacy, sim_pf_sim_whole, sim_pf_init. ss. *)
-(* Qed. *)
-
-(* Lemma self_promise_remove_lifting *)
-(*       lang st1 st2 lc1_src lc1_tgt lc2_tgt mem1_tgt mem2_tgt mem1_src sc1 sc2 P  *)
-(*       (STATE1 : Forget.forget_local lc1_src lc1_tgt) *)
-(*       (MEM1 : Forget.forget_memory (Local.is_promised_loc lc1_src) *)
-(*                                   mem1_src mem1_tgt) *)
-(*       (TGT_STEP : tau (@pred_step P _)  *)
-(*                       (Thread.mk lang st1 lc1_tgt sc1 mem1_tgt) *)
-(*                       (Thread.mk _ st2 lc2_tgt sc2 mem2_tgt)) *)
-(*       (CONSISTENT : promise_view_consistent lc2_tgt) *)
-(*   : *)
-(*     exists lc2_src mem2_src, *)
-(*       <<SRC_STEP : (rc (tau (@pred_step P _))) *)
-(*                        (Thread.mk _ st1 lc1_src sc1 mem1_src) *)
-(*                        (Thread.mk _ st2 lc2_src sc2 mem2_src)>> /\ *)
-(*       <<STATE1 : Forget.forget_local lc2_src lc2_tgt>> /\ *)
-(*       <<MEM1 : Forget.forget_memory (Local.is_promised_loc lc2_src) *)
-(*                                     mem2_src mem2_tgt>> *)
-(* . *)
-(* Proof. *)
-(*   destruct TGT_STEP, TSTEP, STEP. *)
-(*   dependent destruction STEP. dependent destruction STEP. *)
-(*   - exists lc1_src, mem1_src. destruct LOCAL. subst. *)
-(*     econs; eauto; [| econs]. *)
-(*     + apply Relation_Operators.r_refl. *)
-(*     + destruct STATE1; econs; eauto. *)
-(*     + destruct MEM1. econs; eauto. admit. *)
-(*   - admit. *)
-(* Admitted. *)
-
-(* Lemma other_promise_remove_lifting *)
-(*       lang st1 st2 lc1 lc2 mem1_tgt mem2_tgt mem1_src sc1 sc2 P proms *)
-(*       (MEM1 : Forget.forget_memory proms mem1_src mem1_tgt) *)
-(*       (TGT_STEP : tau (@pred_step (P /1\ no_read_msgs proms /1\ *)
-(*                                      no_read_msgs proms) _)  *)
-(*                       (Thread.mk lang st1 lc1 sc1 mem1_tgt) *)
-(*                       (Thread.mk _ st2 lc2 sc2 mem2_tgt)) *)
-(*   : *)
-(*     exists mem2_src, *)
-(*       <<SRC_STEP : tau (@pred_step (P /1\ no_read_msgs proms /1\ *)
-(*                                       no_read_msgs proms) _)   *)
-(*                        (Thread.mk _ st1 lc1 sc1 mem1_src) *)
-(*                        (Thread.mk _ st2 lc2 sc2 mem2_src)>> /\ *)
-(*       <<MEM1 : Forget.forget_memory proms mem2_src mem2_tgt>> *)
-(* . *)
-(* Admitted. *)
-
-(* Lemma future_lifting *)
-(*       lang st1 st2 lc1 lc2 mem1_tgt mem2_tgt mem1_src sc1 sc2 P v1 v2 *)
-(*       (TGT_STEP : rtc (tau (@pred_step (P /1\ write_between v1 v2) _))  *)
-(*                       (Thread.mk lang st1 lc1 sc1 mem1_tgt) *)
-(*                       (Thread.mk _ st2 lc2 sc2 mem2_tgt)) *)
-(*       (INTERVAL_EMPTY : empty_interval v1 v2 (fun _ => True) mem1_src) *)
-(*       (FUTURE : Memory.le mem1_src mem1_tgt) *)
-(*   : *)
-(*     exists mem2_src, *)
-(*       <<SRC_STEP : rtc (tau (@pred_step (P /1\ write_between v1 v2) _)) *)
-(*                        (Thread.mk _ st1 lc1 sc1 mem1_src) *)
-(*                        (Thread.mk _ st2 lc2 sc2 mem2_src)>> *)
-(* . *)
-(* Admitted. *)
-
+Lemma init_pf s tid st lc
+      (TID: IdentMap.find tid (Threads.init s) = Some (st, lc))
+  :
+    Local.promises lc = Memory.bot.
+Proof.
+  unfold Threads.init in *. erewrite UsualFMapPositive.UsualPositiveMap.Facts.map_o in *.
+  unfold option_map in *. des_ifs.
+Qed.  
+  
+Lemma sim_pf_init
+      s
+      (RACEFREE: pf_racefree (Configuration.init s))
+  :
+    sim_pf_all (Configuration.init s) (Configuration.init s)
+.
+Proof.
+  econs. instantiate (1:=fun _ _ _ => False). instantiate (1:=fun _ => Memory.init).
+  econs; eauto; ss; i.
+  - econs; i; ss.
+    + unfold Threads.init in *. erewrite UsualFMapPositive.UsualPositiveMap.Facts.map_o in *.
+      unfold option_map in *. des_ifs.      
+    + econs.
+      * instantiate (1:= Memory.init). econs; ss; eauto.
+        ii. inv PROMS. ss.
+        exploit init_pf; eauto. i. rewrite x0 in *.
+        inv PROMISED. rewrite Memory.bot_get in *. clarify.
+      * refl.
+  - econs; s.
+    + i. exploit init_pf; try apply TIDTGT; eauto. i.
+      rewrite x0 in *. inv PROM.
+      rewrite Memory.bot_get in *. clarify.
+    + i. clarify.
+  - econs; eauto. refl.
+  - eapply Configuration.init_wf.
+  - eapply Configuration.init_wf.
+Qed. 
