src/drf/Race.v
@@ -23,20 +23,31 @@ Require Import PF.
 Set Implicit Arguments.
 
 
+(* TODO unifiy and remove definitions in Event.v *)
+Definition ProgramEvent_is_updating (e:ProgramEvent.t): option (Loc.t * Const.t * Ordering.t) :=
+  match e with
+  | ProgramEvent.update loc valr _ ordr _ => Some (loc, valr, ordr)
+  | _ => None
+  end.
+
+Inductive pf_race_condition e1 e2: Prop :=
+| pf_race_condition_rw
+    loc val1 val2 ordr ordw
+    (EVENT1: ProgramEvent.is_reading e1 = Some (loc, val1, ordr))
+    (EVENT2: ProgramEvent.is_writing e2 = Some (loc, val2, ordw))
+    (ORDW: Ordering.le ordw Ordering.relaxed)
+| pf_race_condition_uu
+    loc val1 val2 ordu1 ordu2
+    (EVENT1: ProgramEvent_is_updating e1 = Some (loc, val1, ordu1))
+    (EVENT2: ProgramEvent_is_updating e2 = Some (loc, val2, ordu2))
+    (ORDU: Ordering.le ordu1 Ordering.relaxed \/ Ordering.le ordu2 Ordering.relaxed)
+.
+Hint Constructors pf_race_condition.
+
 Definition can_step lang (st : Language.state lang) (e : ProgramEvent.t) : Prop :=
   exists st', Language.step _ e st st'.
 
-Inductive race_condition e1 e2 ord1 ord2 : Prop :=
-| race_condition_rw loc val1 val2
-    (EVENT1: ProgramEvent.is_reading e1 = Some (loc, val1, ord1))
-    (EVENT2: ProgramEvent.is_writing e2 = Some (loc, val2, ord2))
-| race_condition_ww loc val1 val2
-    (EVENT1: ProgramEvent.is_writing e1 = Some (loc, val1, ord1))
-    (EVENT2: ProgramEvent.is_writing e2 = Some (loc, val2, ord2))
-.
-Hint Constructors race_condition.
-
-Inductive race (c:Configuration.t) (ord1 ord2:Ordering.t): Prop :=
+Inductive pf_race (c:Configuration.t): Prop :=
 | race_intro
     tid1 e1 lang1 st1 lc1
     tid2 e2 lang2 st2 lc2
@@ -45,25 +56,22 @@ Inductive race (c:Configuration.t) (ord1 ord2:Ordering.t): Prop :=
     (TIDDIFF: tid1 <> tid2)
     (PROEVT1: can_step _ st1 e1)
     (PROEVT2: can_step _ st2 e2)
-    (RACE: race_condition e1 e2 ord1 ord2)
+    (RACE: pf_race_condition e1 e2)
 .
-Hint Constructors race.
+Hint Constructors pf_race.
 
 Definition pf_racefree (c1:Configuration.t): Prop :=
-  forall c2 ordr ordw
-         (STEPS: rtc pftstep_all c1 c2),
-    (<<RACEFREE: forall (RACE: race c2 ordr ordw),
-        (<<ORDR: Ordering.le Ordering.acqrel ordr>>) /\
-        (<<ORDW: Ordering.le Ordering.acqrel ordw>>)>>)
-.
+  forall c2
+         (STEPS: rtc pftstep_all c1 c2)
+         (RACE: pf_race c2), False.
 
 Lemma pf_racefree_step c1 c2
       (RACEFREE : pf_racefree c1)
       (STEP : rtc pftstep_all c1 c2) :
   pf_racefree c2.
 Proof.
-  intros c3 ordr ordw STEPS.
-  apply (RACEFREE c3); etrans; eauto.
+  intros c3 STEPS RACE.
+  apply (RACEFREE c3); auto. etrans; eauto.
 Qed.
 
 Definition is_reading lang (st : Language.state lang) l o :=
@@ -75,3 +83,8 @@ Definition is_writing lang (st : Language.state lang) l o :=
   exists e v o', can_step _ st e /\
                  Ordering.le o' o /\
                  ProgramEvent.is_writing e = Some (l, v, o').
+
+Definition is_updating lang (st : Language.state lang) l o :=
+  exists e v o', can_step _ st e /\
+                 Ordering.le o' o /\
+                 ProgramEvent_is_updating e = Some (l, v, o').
